src/tls/test/TestClient.fst
@@ -11,6 +11,8 @@ open TLSConstants
 open TLSInfo
 open StatefulLHAE
 
+(* FlexRecord *)
+
 let config =
     let sigPref = [CoreCrypto.RSASIG] in
     let hashPref = [Hash CoreCrypto.SHA256] in
@@ -26,7 +28,7 @@ let config =
 
 let id = {
     msId = noMsId;
-    kdfAlg = PRF_SSL3_nested;
+    kdfAlg = PRF_TLS_1p2 kdf_label (HMAC CoreCrypto.SHA256);
     pv = TLS_1p2;
     aeAlg = (AEAD CoreCrypto.AES_128_GCM CoreCrypto.SHA256);
     csrConn = bytes_of_hex "";
@@ -96,7 +98,6 @@ let encryptRecord_TLS12_AES_GCM_128_SHA256 w ct plain =
   // FIXME: without the three additional #-arguments below, extraction crashes
   StatefulLHAE.encrypt #id #ad #rg w f
 
-
 let decryptRecord_TLS12_AES_GCM_128_SHA256 rd ct cipher = 
   let ad: StatefulPlain.adata id = StatefulPlain.makeAD id ct in
   let (Some d) = StatefulLHAE.decrypt #id #ad rd cipher in
@@ -105,10 +106,14 @@ let decryptRecord_TLS12_AES_GCM_128_SHA256 rd ct cipher =
 (* We should use Content.mk_fragment |> Content.repr, not Record.makePacket *)
 (* Even better, we should move to TLS.send *)
 
-let sendHSRecord tcp pv log hs_msg = 
-  let r = Record.makePacket Content.Handshake pv hs_msg in
+let sendRecord tcp pv ct msg str = 
+  let r = Record.makePacket ct pv msg in
   let Correct _ = Platform.Tcp.send tcp r in
-  log @| hs_msg
+  match ct with
+  | Content.Application_data ->   IO.print_string ("Sending Data("^str^")\n")
+  | Content.Handshake ->   IO.print_string ("Sending HS("^str^")\n")
+  | Content.Change_cipher_spec ->   IO.print_string ("Sending CCS\n")
+  | Content.Alert ->   IO.print_string ("Sending Alert("^str^")\n")
 
 val really_read_rec: bytes -> Platform.Tcp.networkStream -> nat -> optResult string bytes
 let rec really_read_rec prev tcp len = 
@@ -124,71 +129,54 @@ let rec really_read_rec prev tcp len =
       
 let really_read = really_read_rec empty_bytes
 
-val recvHSRecordRec: bytes -> Platform.Tcp.networkStream -> protocolVersion -> kexAlg -> bytes -> (hs_msg * bytes)
-let rec recvHSRecordRec prev tcp pv kex log = 
-//  IO.print_string (Platform.Bytes.print_bytes prev);
-//  IO.print_string ((string_of_int (length prev))^" left from before\n");
+let recvRecord tcp pv = 
   match really_read tcp 5 with 
   | Correct header ->
       match Record.parseHeader header with  
-      | Correct (Content.Handshake,pv,len)  ->
-         IO.print_string ((string_of_int len)^" bytes expected\n");
+      | Correct (ct,pv,len)  ->
          match really_read tcp len  with
-         | Correct payload -> 
-	      let buf = prev @| payload in 
-	      let Correct (rem,hsm) = Handshake.parseHandshakeMessages (Some pv) (Some kex) buf in 
-	      //IO.print_string ((string_of_int (List.Tot.length hsm))^" messages\n");
-	      //IO.print_string ((string_of_int (length rem))^" left\n");
-	      (match hsm with 
-	      | [] -> recvHSRecordRec rem tcp pv kex log 
-	      | [(hs_msg,to_log)] ->  hs_msg, log @| to_log)
+         | Correct payload -> (ct,pv,payload)
 
-let recvHSRecord = recvHSRecordRec empty_bytes
+let makeHSRecord pv hs_msg log =
+  let hs = HandshakeMessages.handshakeMessageBytes pv hs_msg in
+  (string_of_handshakeMessage hs_msg,hs,log@|hs)
 
-let sendAppDataRecord tcp pv msg = 
-  let r = Record.makePacket Content.Application_data pv msg in
-  let Correct _ = Platform.Tcp.send tcp r in
-  ()
+let sendHSRecord tcp pv hs_msg log = 
+  let (str,hs,log) = makeHSRecord pv hs_msg log in
+  sendRecord tcp pv Content.Handshake hs str;
+  log
 
-let sendCCSRecord tcp pv = 
-  let r = Record.makePacket Content.Change_cipher_spec pv HandshakeMessages.ccsBytes in
-  let Correct _ = Platform.Tcp.send tcp r in
-  ()
-  
+let recvHSRecord tcp pv kex log = 
+  let (Content.Handshake,rpv,pl) = recvRecord tcp pv in
+  let Correct (rem,[(hs_msg,to_log)]) = Handshake.parseHandshakeMessages (Some pv) (Some kex) pl in 
+  IO.print_string ("Received HS("^(string_of_handshakeMessage hs_msg)^")\n");
+  (hs_msg,log @| to_log)
+
 let recvCCSRecord tcp pv = 
-  match really_read tcp 5 with 
-  | Correct header ->
-      match Record.parseHeader header with  
-      | Correct (Content.Change_cipher_spec,pv,len)  ->
-         match really_read tcp len  with
-         | Correct cipher -> cipher
-
+  let (Content.Change_cipher_spec,_,ccs) = recvRecord tcp pv in
+  IO.print_string "Received CCS\n";
+  ccs
 
 let recvEncHSRecord tcp pv kex log rd = 
-  match really_read tcp 5 with 
-  | Correct header ->
-      match Record.parseHeader header with  
-      | Correct (Content.Handshake,pv,len)  ->
-         match really_read tcp len  with
-         | Correct cipher -> 
-	      let payload = decryptRecord_TLS12_AES_GCM_128_SHA256 rd Content.Handshake cipher in
-	      let Correct (rem,hsm) = Handshake.parseHandshakeMessages (Some pv) (Some kex) payload in
-     	      let [(hs_msg,to_log)] = hsm in
-	      hs_msg, log @| to_log	      
-
+  let (Content.Handshake,_,cipher) = recvRecord tcp pv in
+  let payload = decryptRecord_TLS12_AES_GCM_128_SHA256 rd Content.Handshake cipher in
+  let Correct (rem,hsm) = Handshake.parseHandshakeMessages (Some pv) (Some kex) payload in
+  let [(hs_msg,to_log)] = hsm in
+  IO.print_string ("Received HS("^(string_of_handshakeMessage hs_msg)^")\n");
+  hs_msg, log @| to_log	      
 
 let recvEncAppDataRecord tcp pv rd = 
-  match really_read tcp 5 with 
-  | Correct header ->
-      match Record.parseHeader header with  
-      | Correct (Content.Application_data,pv,len)  ->
-         match really_read tcp len  with
-         | Correct cipher -> 
-	      let payload = decryptRecord_TLS12_AES_GCM_128_SHA256 rd Content.Application_data cipher in
-	      payload
+  let (Content.Application_data,_,cipher) = recvRecord tcp pv in
+  let payload = decryptRecord_TLS12_AES_GCM_128_SHA256 rd Content.Application_data cipher in
+  IO.print_string "Received Data:\n";
+  IO.print_string ((iutf8 payload)^"\n");
+  payload
+
+(* Flex Handshake *)
+
 
 let deriveKeys_TLS12_AES_GCM_128_SHA256 ms cr sr = 
-  let b = TLSPRF.kdf (PRF_TLS_1p2 kdf_label ((HMAC CoreCrypto.SHA256))) ms (sr @| cr) 40 in
+  let b = TLSPRF.kdf id.kdfAlg ms (sr @| cr) 40 in
   let cekb, b = split b 16 in
   let sekb, b = split b 16 in
   let civb, sivb = split b 4 in
@@ -200,46 +188,28 @@ let main host port =
   let tcp = Platform.Tcp.connect host port in
   let log = empty_bytes in
   
-(*
-  let st = Handshake.init Client ... in
-  Handhake.send_client_hello st;
-  let chb = Handshake.next_message st in
-*)
-
-
   let (None,ch,chb) = Handshake.prepareClientHello config None None in
   let pv = ch.ch_protocol_version in 
   let kex = TLSConstants.Kex_ECDHE in
-
-  IO.print_string "Sending ClientHello\n";
-  let log = sendHSRecord tcp pv log chb in
+  let log = sendHSRecord tcp pv (ClientHello ch) log in
 
   let ServerHello(sh),log = recvHSRecord tcp pv kex log in
-  IO.print_string "Received ServerHello\n";
 
   let pv = sh.sh_protocol_version in
   let cs = sh.sh_cipher_suite in
   let CipherSuite kex sa ae = cs in
 
   let Certificate(sc),log = recvHSRecord tcp pv kex log in
-  IO.print_string "Received ServerCertificate\n";
-
   let ServerKeyExchange(ske),log = recvHSRecord tcp pv kex log in
-  IO.print_string "Received ServerKeyExchange\n";
-
   let ServerHelloDone,log = recvHSRecord tcp pv kex log in
-  IO.print_string "Received ServerHelloDone\n";
 
   let KEX_S_DHE gy = ske.ske_kex_s in
   let gx, pms = CommonDH.dh_responder gy in
   let cke = {cke_kex_c = kex_c_of_dh_key gx} in
-  let ckeb = clientKeyExchangeBytes sh.sh_protocol_version cke in
-  IO.print_string "Sending ClientKeyExchange\n";
-  let log = sendHSRecord tcp pv log ckeb in
+  let log = sendHSRecord tcp pv (ClientKeyExchange cke) log in
 
   let ms = TLSPRF.prf (pv,cs) pms (utf8 "master secret") (ch.ch_client_random @| sh.sh_server_random)  48 in
   IO.print_string ("master secret:"^(Platform.Bytes.print_bytes ms)^"\n");
-
   let (ck,civ,sk,siv) = deriveKeys_TLS12_AES_GCM_128_SHA256 ms ch.ch_client_random sh.sh_server_random in
   IO.print_string ("client AES_GCM write key:"^(Platform.Bytes.print_bytes ck)^"\n");
   IO.print_string ("client AES_GCM salt: iv:"^(Platform.Bytes.print_bytes civ)^"\n");
@@ -248,28 +218,24 @@ let main host port =
   let wr = encryptor_TLS12_AES_GCM_128_SHA256 ck civ in
   let rd = decryptor_TLS12_AES_GCM_128_SHA256 sk siv in
 
-
-  IO.print_string "Sending ClientCCS\n";
-  sendCCSRecord tcp pv;
-
   let cfin = {fin_vd = TLSPRF.verifyData (pv,cs) ms Client log} in 
-  let cfinb = finishedBytes cfin in
+  let (str,cfinb,log) = makeHSRecord pv (Finished cfin) log in
   let efinb = encryptRecord_TLS12_AES_GCM_128_SHA256 wr Content.Handshake cfinb in
-  IO.print_string "Sending ClientFinished\n";
 
-  let log = sendHSRecord tcp pv log efinb in
+  sendRecord tcp pv Content.Change_cipher_spec HandshakeMessages.ccsBytes "Client";
+  sendRecord tcp pv Content.Handshake efinb str;
 
   let _ = recvCCSRecord tcp pv in
-
-  IO.print_string "Received ServerCCS\n";
   let Finished(sfin),log = recvEncHSRecord tcp pv kex log rd in
-  IO.print_string "Received ServerFinished\n";
+
   let payload = "GET / HTTP/1.1\r\nHost: " ^ host ^ "\r\n\r\n" in
   let get = encryptRecord_TLS12_AES_GCM_128_SHA256 wr Content.Application_data (utf8 payload) in
-  IO.print_string "Sending AppData(GET /)\n";
-  sendAppDataRecord tcp pv get;
+
+  sendRecord tcp pv Content.Application_data get "GET /";
   let ad = recvEncAppDataRecord tcp pv rd in
-  IO.print_string "Received AppData:\n";
-  IO.print_string ((iutf8 ad)^"\n");
   ()
+
   
+
+
+
